Some consistency/robustness tweaks.
- Name all variables that we refer to.
- Put types in definitions.

theories/infinite.v
@@ -12,83 +12,74 @@ Class Infinite A :=
 Instance string_infinite: Infinite string := {| inject := λ x, "~" +:+ pretty x |}.
 Instance nat_infinite: Infinite nat := {| inject := id |}.
 Instance N_infinite: Infinite N := {| inject_injective := Nat2N.inj |}.
-Instance pos_infinite: Infinite positive := {| inject_injective := SuccNat2Pos.inj |}.
+Instance positive_infinite: Infinite positive := {| inject_injective := SuccNat2Pos.inj |}.
 Instance Z_infinite: Infinite Z := {| inject_injective := Nat2Z.inj |}.
+
 Instance option_infinite `{Infinite A}: Infinite (option A) := {| inject := Some ∘ inject |}.
 Program Instance list_infinite `{Inhabited A}: Infinite (list A) :=
   {| inject := λ i, replicate i inhabitant |}.
 Next Obligation.
 Proof.
-  intros * i j eqrep%(f_equal length).
-  rewrite !replicate_length in eqrep; done.
+  intros A * i j Heqrep%(f_equal length).
+  rewrite !replicate_length in Heqrep; done.
 Qed.
 
 (** * Fresh elements *)
 Section Fresh.
-  Context `{FinCollection A C} `{Infinite A, !RelDecision (@elem_of A C _)}.
+  Context `{FinCollection A C, Infinite A, !RelDecision (@elem_of A C _)}.
 
-  Definition fresh_generic_body (s: C) (rec: ∀ s', s' ⊂ s → nat → A) (n: nat) :=
+  Definition fresh_generic_body (s : C) (rec : ∀ s', s' ⊂ s → nat → A) (n : nat) : A :=
     let cand := inject n in
     match decide (cand ∈ s) with
     | left H => rec _ (subset_difference_elem_of H) (S n)
     | right _ => cand
     end.
-  Lemma fresh_generic_body_proper s (f g: ∀ y, y ⊂ s → nat → A):
-    (∀ y Hy Hy', pointwise_relation nat eq (f y Hy) (g y Hy')) →
-    pointwise_relation nat eq (fresh_generic_body s f) (fresh_generic_body s g).
+
+  Definition fresh_generic_fix : C → nat → A :=
+    Fix (wf_guard 20 collection_wf) (const (nat → A)) fresh_generic_body.
+
+  Lemma fresh_generic_fixpoint_unfold s n:
+    fresh_generic_fix s n = fresh_generic_body s (λ s' _, fresh_generic_fix s') n.
   Proof.
-    intros relfg i.
-    unfold fresh_generic_body.
-    destruct decide; auto.
-    apply relfg.
+    refine (Fix_unfold_rel _ _ (const (pointwise_relation nat (=))) _ _ s n).
+    intros s' f g Hfg i. unfold fresh_generic_body. case_decide; naive_solver.
   Qed.
 
-  Definition fresh_generic_fix u :=
-    Fix (wf_guard u collection_wf) (const (nat → A)) fresh_generic_body.
-
-  Lemma fresh_generic_fixpoint_unfold u s n:
-    fresh_generic_fix u s n = fresh_generic_body s (λ s' _ n, fresh_generic_fix u s' n) n.
-  Proof.
-    apply (Fix_unfold_rel (wf_guard u collection_wf)
-                          (const (nat → A)) (const (pointwise_relation nat (=)))
-                          fresh_generic_body fresh_generic_body_proper s n).
-  Qed.
-
-  Lemma fresh_generic_fixpoint_spec u s n:
-    ∃ m, n ≤ m ∧ fresh_generic_fix u s n = inject m ∧ inject m ∉ s ∧ ∀ i, n ≤ i < m → inject i ∈ s.
+  Lemma fresh_generic_fixpoint_spec s n :
+    ∃ m, n ≤ m ∧ fresh_generic_fix s n = inject m ∧ inject m ∉ s ∧
+         ∀ i, n ≤ i < m → inject i ∈ s.
   Proof.
     revert n.
-    induction s as [s IH] using (well_founded_ind collection_wf); intro.
+    induction s as [s IH] using (well_founded_ind collection_wf); intros n.
     setoid_rewrite fresh_generic_fixpoint_unfold; unfold fresh_generic_body.
-    destruct decide as [case|case]; eauto with omega.
-    destruct (IH _ (subset_difference_elem_of case) (S n)) as [m [mbound [eqfix [notin inbelow]]]].
+    destruct decide as [Hcase|Hcase]; [|by eauto with omega].
+    destruct (IH _ (subset_difference_elem_of Hcase) (S n))
+      as (m & Hmbound & Heqfix & Hnotin & Hinbelow).
     exists m; repeat split; auto with omega.
-    - rewrite not_elem_of_difference, elem_of_singleton in notin.
-      destruct notin as [?|?%inject_injective]; auto with omega.
-    - intros i ibound.
-      destruct (decide (i = n)) as [<-|neq]; auto.
-      enough (inject i ∈ s ∖ {[inject n]}) by set_solver.
-      apply inbelow; omega.
+    - rewrite not_elem_of_difference, elem_of_singleton in Hnotin.
+      destruct Hnotin as [?|?%inject_injective]; auto with omega.
+    - intros i Hibound.
+      destruct (decide (i = n)) as [<-|Hneq]; [by auto|].
+      assert (inject i ∈ s ∖ {[inject n]}) by auto with omega.
+      set_solver.
   Qed.
 
-  Instance fresh_generic: Fresh A C := λ s, fresh_generic_fix 20 s 0.
+  Instance fresh_generic : Fresh A C := λ s, fresh_generic_fix s 0.
 
-  Instance fresh_generic_spec: FreshSpec A C.
+  Instance fresh_generic_spec : FreshSpec A C.
   Proof.
     split.
     - apply _.
-    - intros * eqXY.
-      unfold fresh, fresh_generic.
-      destruct (fresh_generic_fixpoint_spec 20 X 0)
-        as [mX [_ [-> [notinX belowinX]]]].
-      destruct (fresh_generic_fixpoint_spec 20 Y 0)
-        as [mY [_ [-> [notinY belowinY]]]].
+    - intros X Y HeqXY. unfold fresh, fresh_generic.
+      destruct (fresh_generic_fixpoint_spec X 0)
+        as (mX & _ & -> & HnotinX & HbelowinX).
+      destruct (fresh_generic_fixpoint_spec Y 0)
+        as (mY & _ & -> & HnotinY & HbelowinY).
       destruct (Nat.lt_trichotomy mX mY) as [case|[->|case]]; auto.
-      + contradict notinX; rewrite eqXY; apply belowinY; omega.
-      + contradict notinY; rewrite <- eqXY; apply belowinX; omega.
-    - intro.
-      unfold fresh, fresh_generic.
-      destruct (fresh_generic_fixpoint_spec 20 X 0)
-        as [m [_ [-> [notinX belowinX]]]]; auto.
+      + contradict HnotinX. rewrite HeqXY. apply HbelowinY; omega.
+      + contradict HnotinY. rewrite <-HeqXY. apply HbelowinX; omega.
+    - intros X. unfold fresh, fresh_generic.
+      destruct (fresh_generic_fixpoint_spec X 0)
+        as (m & _ & -> & HnotinX & HbelowinX); auto.
   Qed.
 End Fresh.
